@base <http://iec.ch/TC57/2013/CIM-schema-cim16#> .
@prefix rdf: <http://www.w3.org/1999/02/22-rdf-syntax-ns#> .
@prefix rdfs: <http://www.w3.org/2000/01/rdf-schema#> .
@prefix xsd: <http://www.w3.org/2001/XMLSchema#> .

<IdentifiedObject> rdf:type rdfs:Class ;
	rdfs:label "IdentifiedObject"@en ;
	rdfs:comment "This is a root class to provide common identification for all classes needing identification and naming attributes."^^rdf:XMLLiteral .
<IdentifiedObject.description> rdf:type rdfs:Property ;
	rdfs:label "description"@en ;
	rdfs:domain <IdentifiedObject> ;
	rdfs:range xsd:string ;
	rdfs:comment "The description is a free human readable text describing or naming the object. It may be non unique and may not correlate to a naming hierarchy."^^rdf:XMLLiteral .
<IdentifiedObject.mRID> rdf:type rdfs:Property ;
	rdfs:label "mRID"@en ;
	rdfs:domain <IdentifiedObject> ;
	rdfs:range xsd:string ;
	rdfs:comment "Master resource identifier issued by a model authority. The mRID is unique within an exchange context. Global uniqueness is easily achieved by using a UUID, as specified in RFC 4122, for the mRID. The use of UUID is strongly recommended.\nFor CIMXML data files in RDF syntax conforming to IEC 61970-552, the mRID is mapped to rdf:ID or rdf:about attributes that identify CIM object elements."^^rdf:XMLLiteral .
<IdentifiedObject.name> rdf:type rdfs:Property ;
	rdfs:label "name"@en ;
	rdfs:domain <IdentifiedObject> ;
	rdfs:range xsd:string ;
	rdfs:comment "The name is any free human readable and possibly non unique text naming the object."^^rdf:XMLLiteral .

<Curve> rdf:type rdfs:Class ;
	rdfs:subClassOf <IdentifiedObject> ;
	rdfs:label "Curve"@en ;
	rdfs:comment "A multi-purpose curve or functional relationship between an independent variable (X-axis) and dependent (Y-axis) variables. "^^rdf:XMLLiteral .
<Curve.curveStyle> rdf:type rdfs:Property ;
	rdfs:label "curveStyle"@en ;
	rdfs:domain <Curve> ;
	rdfs:range xsd:string ;
	rdfs:comment "The style or shape of the curve."^^rdf:XMLLiteral .
<Curve.xMultiplier> rdf:type rdfs:Property ;
	rdfs:label "xMultiplier"@en ;
	rdfs:domain <Curve> ;
	rdfs:range xsd:string ;
	rdfs:comment "Multiplier for X-axis."^^rdf:XMLLiteral .
<Curve.xUnit> rdf:type rdfs:Property ;
	rdfs:label "xUnit"@en ;
	rdfs:domain <Curve> ;
	rdfs:range xsd:string ;
	rdfs:comment "The X-axis units of measure."^^rdf:XMLLiteral .
<Curve.y1Multiplier> rdf:type rdfs:Property ;
	rdfs:label "y1Multiplier"@en ;
	rdfs:domain <Curve> ;
	rdfs:range xsd:string ;
	rdfs:comment "Multiplier for Y1-axis."^^rdf:XMLLiteral .
<Curve.y1Unit> rdf:type rdfs:Property ;
	rdfs:label "y1Unit"@en ;
	rdfs:domain <Curve> ;
	rdfs:range xsd:string ;
	rdfs:comment "The Y1-axis units of measure."^^rdf:XMLLiteral .
<Curve.y2Multiplier> rdf:type rdfs:Property ;
	rdfs:label "y2Multiplier"@en ;
	rdfs:domain <Curve> ;
	rdfs:range xsd:string ;
	rdfs:comment "Multiplier for Y2-axis."^^rdf:XMLLiteral .
<Curve.y2Unit> rdf:type rdfs:Property ;
	rdfs:label "y2Unit"@en ;
	rdfs:domain <Curve> ;
	rdfs:range xsd:string ;
	rdfs:comment "The Y2-axis units of measure."^^rdf:XMLLiteral .
<Curve.y3Multiplier> rdf:type rdfs:Property ;
	rdfs:label "y3Multiplier"@en ;
	rdfs:domain <Curve> ;
	rdfs:range xsd:string ;
	rdfs:comment "Multiplier for Y3-axis."^^rdf:XMLLiteral .
<Curve.y3Unit> rdf:type rdfs:Property ;
	rdfs:label "y3Unit"@en ;
	rdfs:domain <Curve> ;
	rdfs:range xsd:string ;
	rdfs:comment "The Y3-axis units of measure."^^rdf:XMLLiteral .
<Curve.CurveDatas> rdf:type rdfs:Property ;
	rdfs:label "CurveDatas"@en ;
	rdfs:domain <Curve> ;
	rdfs:range <CurveData> ;
	rdfs:comment "The point data values that define this curve."^^rdf:XMLLiteral .

<StringFixedLanguage> rdf:type rdfs:Datatype ;
	rdfs:label "StringFixedLanguage"@en ;
	rdfs:comment "A string consisting of a sequence of characters. The character encoding is UTF-8. The string length is unspecified and unlimited.\nThe primitive is serialized as literal without language support."^^rdf:XMLLiteral .

<SimulationSettings> rdf:type rdfs:Class ;
	rdfs:subClassOf <IdentifiedObject> ;
	rdfs:label "SimulationSettings"@en ;
	rdfs:comment "Describes simulation settings necessary for a simulation."^^rdf:XMLLiteral .
<SimulationSettings.SimulationResult> rdf:type rdfs:Property ;
	rdfs:label "SimulationResult"@en ;
	rdfs:domain <SimulationSettings> ;
	rdfs:range <SimulationResult> ;
	rdfs:comment "The simulation reslut to which this simulation settings belong to."^^rdf:XMLLiteral .

<SignalConfiguration> rdf:type rdfs:Class ;
	rdfs:subClassOf <IdentifiedObject> ;
	rdfs:label "SignalConfiguration"@en ;
	rdfs:comment "A configuration or a set of signals selected for recording during a simulation."^^rdf:XMLLiteral .
<SignalConfiguration.SimulationResult> rdf:type rdfs:Property ;
	rdfs:label "SimulationResult"@en ;
	rdfs:domain <SignalConfiguration> ;
	rdfs:range <SimulationResult> ;
	rdfs:comment "The simulation reslut to which this simulation configuration belongs to."^^rdf:XMLLiteral .

<SimulationEvents> rdf:type rdfs:Class ;
	rdfs:subClassOf <IdentifiedObject> ;
	rdfs:label "SimulationEvents"@en ;
	rdfs:comment "A configuration or a set of events executed during a simulation."^^rdf:XMLLiteral .
<SimulationEvents.SimulationResult> rdf:type rdfs:Property ;
	rdfs:label "SimulationResult"@en ;
	rdfs:domain <SimulationEvents> ;
	rdfs:range <SimulationResult> ;
	rdfs:comment "The simulation reslut to which this simulation events belong to."^^rdf:XMLLiteral .

<CurveData> rdf:type rdfs:Class ;
	rdfs:label "CurveData"@en ;
	rdfs:comment "Multi-purpose data points for defining a curve.  The use of this generic class is discouraged if a more specific class can be used to specify the X and Y axis values along with their specific data types."^^rdf:XMLLiteral .
<CurveData.xvalue> rdf:type rdfs:Property ;
	rdfs:label "xvalue"@en ;
	rdfs:domain <CurveData> ;
	rdfs:range xsd:double ;
	rdfs:comment "The data value of the X-axis variable,  depending on the X-axis units."^^rdf:XMLLiteral .
<CurveData.y1value> rdf:type rdfs:Property ;
	rdfs:label "y1value"@en ;
	rdfs:domain <CurveData> ;
	rdfs:range xsd:double ;
	rdfs:comment "The data value of the  first Y-axis variable, depending on the Y-axis units."^^rdf:XMLLiteral .
<CurveData.y2value> rdf:type rdfs:Property ;
	rdfs:label "y2value"@en ;
	rdfs:domain <CurveData> ;
	rdfs:range xsd:double ;
	rdfs:comment "The data value of the second Y-axis variable (if present), depending on the Y-axis units."^^rdf:XMLLiteral .
<CurveData.y3value> rdf:type rdfs:Property ;
	rdfs:label "y3value"@en ;
	rdfs:domain <CurveData> ;
	rdfs:range xsd:double ;
	rdfs:comment "The data value of the third Y-axis variable (if present), depending on the Y-axis units."^^rdf:XMLLiteral .
<CurveData.Curve> rdf:type rdfs:Property ;
	rdfs:label "Curve"@en ;
	rdfs:domain <CurveData> ;
	rdfs:range <Curve> ;
	rdfs:comment "The curve of  this curve data point."^^rdf:XMLLiteral .

<SimulationResultCharacteristic> rdf:type rdfs:Class ;
	rdfs:subClassOf <Curve> ;
	rdfs:label "SimulationResultCharacteristic"@en ;
	rdfs:comment "Result characteristic. The xvalue of the curve is time."^^rdf:XMLLiteral .
<SimulationResultCharacteristic.resultReference> rdf:type rdfs:Property ;
	rdfs:label "resultReference"@en ;
	rdfs:domain <SimulationResultCharacteristic> ;
	rdfs:range <IRI> ;
	rdfs:comment "Reference to an artifact containing the data for the characteristic. This can be a reference to comma separated file or other serialization."^^rdf:XMLLiteral .
<SimulationResultCharacteristic.y2valueSignal> rdf:type rdfs:Property ;
	rdfs:label "y2valueSignal"@en ;
	rdfs:domain <SimulationResultCharacteristic> ;
	rdfs:range <SignalRecorder> ;
	rdfs:comment "The signal for y2value of the characteristic."^^rdf:XMLLiteral .
<SimulationResultCharacteristic.y1valueSignal> rdf:type rdfs:Property ;
	rdfs:label "y1valueSignal"@en ;
	rdfs:domain <SimulationResultCharacteristic> ;
	rdfs:range <SignalRecorder> ;
	rdfs:comment "The signal for y1value of the characteristic."^^rdf:XMLLiteral .
<SimulationResultCharacteristic.SimulationResult> rdf:type rdfs:Property ;
	rdfs:label "SimulationResult"@en ;
	rdfs:domain <SimulationResultCharacteristic> ;
	rdfs:range <SimulationResult> ;
	rdfs:comment "The simulation reslut to which this simulation result characteristic belongs to."^^rdf:XMLLiteral .
<SimulationResultCharacteristic.y3valueSignal> rdf:type rdfs:Property ;
	rdfs:label "y3valueSignal"@en ;
	rdfs:domain <SimulationResultCharacteristic> ;
	rdfs:range <SignalRecorder> ;
	rdfs:comment "The signal for y3value of the characteristic."^^rdf:XMLLiteral .

<SignalRecorder> rdf:type rdfs:Class ;
	rdfs:subClassOf <IdentifiedObject> ;
	rdfs:label "SignalRecorder"@en ;
	rdfs:comment "A recorder for a given signal."^^rdf:XMLLiteral .
<SignalRecorder.SimulationChacteristic2> rdf:type rdfs:Property ;
	rdfs:label "SimulationChacteristic2"@en ;
	rdfs:domain <SignalRecorder> ;
	rdfs:range <SimulationResultCharacteristic> ;
	rdfs:comment "The characteristic where this signal is plotted."^^rdf:XMLLiteral .
<SignalRecorder.SimulationCharacteristic1> rdf:type rdfs:Property ;
	rdfs:label "SimulationCharacteristic1"@en ;
	rdfs:domain <SignalRecorder> ;
	rdfs:range <SimulationResultCharacteristic> ;
	rdfs:comment "The characteristic where this signal is plotted."^^rdf:XMLLiteral .
<SignalRecorder.SimulationCharacteristic3> rdf:type rdfs:Property ;
	rdfs:label "SimulationCharacteristic3"@en ;
	rdfs:domain <SignalRecorder> ;
	rdfs:range <SimulationResultCharacteristic> ;
	rdfs:comment "The characteristic where this signal is plotted."^^rdf:XMLLiteral .

<SimulationResult> rdf:type rdfs:Class ;
	rdfs:subClassOf <IdentifiedObject> ;
	rdfs:label "SimulationResult"@en ;
	rdfs:comment "Represents the simulation result."^^rdf:XMLLiteral .
<SimulationResult.SimulationSettings> rdf:type rdfs:Property ;
	rdfs:label "SimulationSettings"@en ;
	rdfs:domain <SimulationResult> ;
	rdfs:range <SimulationSettings> ;
	rdfs:comment "The simulation settings that are part of the simulation result."^^rdf:XMLLiteral .
<SimulationResult.SignalConfiguration> rdf:type rdfs:Property ;
	rdfs:label "SignalConfiguration"@en ;
	rdfs:domain <SimulationResult> ;
	rdfs:range <SignalConfiguration> ;
	rdfs:comment "The simulation configuration that is part of the simulation result."^^rdf:XMLLiteral .
<SimulationResult.SimulationEvents> rdf:type rdfs:Property ;
	rdfs:label "SimulationEvents"@en ;
	rdfs:domain <SimulationResult> ;
	rdfs:range <SimulationEvents> ;
	rdfs:comment "The simulation events that are part of the simulation result."^^rdf:XMLLiteral .
<SimulationResult.SimulationResultCharacteristic> rdf:type rdfs:Property ;
	rdfs:label "SimulationResultCharacteristic"@en ;
	rdfs:domain <SimulationResult> ;
	rdfs:range <SimulationResultCharacteristic> ;
	rdfs:comment "The simulation result characteristic that is part of the simulation result."^^rdf:XMLLiteral .

<IRI> rdf:type rdfs:Datatype ;
	rdfs:label "IRI"@en ;
	rdfs:comment "An IRI (Internationalized Resource Identifier) within an RDF graph is a Unicode string that conforms to the syntax defined in RFC 3987.\nThe primitive is serialized as rdf:resource in RDFXML.\nIRIs in the RDF abstract syntax must be absolute, and may contain a fragment identifier.\nIRI equality: Two IRIs are equal if and only if they are equivalent under Simple String Comparison according to section 5.1 of [RFC3987]. Further normalization must not be performed when comparing IRIs for equality.\nIRIs are a generalization of URIs [RFC3986] that permits a wider range of Unicode characters. Every absolute URI and URL is an IRI, but not every IRI is an URI. When IRIs are used in operations that are only defined for URIs, they must first be converted according to the mapping defined in section 3.1 of [RFC3987]. A notable example is retrieval over the HTTP protocol. The mapping involves UTF-8 encoding of non-ASCII characters, %-encoding of octets not allowed in URIs, and Punycode-encoding of domain names."^^rdf:XMLLiteral .

<StringIRI> rdf:type rdfs:Datatype ;
	rdfs:label "StringIRI"@en ;
	rdfs:comment "An IRI (Internationalized Resource Identifier) within an RDF graph is a Unicode string that conforms to the syntax defined in RFC 3987.\nThe primitive is serialized as literal without language support.\nIRIs in the RDF abstract syntax must be absolute, and may contain a fragment identifier.\nIRI equality: Two IRIs are equal if and only if they are equivalent under Simple String Comparison according to section 5.1 of [RFC3987]. Further normalization must not be performed when comparing IRIs for equality.\nIRIs are a generalization of URIs [RFC3986] that permits a wider range of Unicode characters. Every absolute URI and URL is an IRI, but not every IRI is an URI. When IRIs are used in operations that are only defined for URIs, they must first be converted according to the mapping defined in section 3.1 of [RFC3987]. A notable example is retrieval over the HTTP protocol. The mapping involves UTF-8 encoding of non-ASCII characters, %-encoding of octets not allowed in URIs, and Punycode-encoding of domain names."^^rdf:XMLLiteral .
