@base <http://iec.ch/TC57/2013/CIM-schema-cim16#> .
@prefix rdf: <http://www.w3.org/1999/02/22-rdf-syntax-ns#> .
@prefix rdfs: <http://www.w3.org/2000/01/rdf-schema#> .
@prefix xsd: <http://www.w3.org/2001/XMLSchema#> .

<DetailedModelTypeDynamics> rdf:type rdfs:Class ;
	rdfs:subClassOf <IdentifiedObject> ;
	rdfs:label "DetailedModelTypeDynamics"@en ;
	rdfs:comment "The main class that packages all related to this type of a detailed model. This includes all parameters, functions, signals, etc."^^rdf:XMLLiteral .
<DetailedModelTypeDynamics.DetailedModelDynamics> rdf:type rdfs:Property ;
	rdfs:label "DetailedModelDynamics"@en ;
	rdfs:domain <DetailedModelTypeDynamics> ;
	rdfs:range <DetailedModelDynamics> ;
	rdfs:comment "The detailed model dynamics that has this type of detailed model dynamics."^^rdf:XMLLiteral .

<DetailedModelDescriptor> rdf:type rdfs:Class ;
	rdfs:subClassOf <IdentifiedObject> ;
	rdfs:label "DetailedModelDescriptor"@en ;
	rdfs:comment "Describes different components of a detailed model."^^rdf:XMLLiteral .

<IdentifiedObject> rdf:type rdfs:Class ;
	rdfs:label "IdentifiedObject"@en ;
	rdfs:comment "This is a root class to provide common identification for all classes needing identification and naming attributes."^^rdf:XMLLiteral .
<IdentifiedObject.description> rdf:type rdfs:Property ;
	rdfs:label "description"@en ;
	rdfs:domain <IdentifiedObject> ;
	rdfs:range xsd:string ;
	rdfs:comment "The description is a free human readable text describing or naming the object. It may be non unique and may not correlate to a naming hierarchy."^^rdf:XMLLiteral .
<IdentifiedObject.mRID> rdf:type rdfs:Property ;
	rdfs:label "mRID"@en ;
	rdfs:domain <IdentifiedObject> ;
	rdfs:range xsd:string ;
	rdfs:comment "Master resource identifier issued by a model authority. The mRID is unique within an exchange context. Global uniqueness is easily achieved by using a UUID, as specified in RFC 4122, for the mRID. The use of UUID is strongly recommended.\nFor CIMXML data files in RDF syntax conforming to IEC 61970-552, the mRID is mapped to rdf:ID or rdf:about attributes that identify CIM object elements."^^rdf:XMLLiteral .
<IdentifiedObject.name> rdf:type rdfs:Property ;
	rdfs:label "name"@en ;
	rdfs:domain <IdentifiedObject> ;
	rdfs:range xsd:string ;
	rdfs:comment "The name is any free human readable and possibly non unique text naming the object."^^rdf:XMLLiteral .

<ParameterValue> rdf:type rdfs:Class ;
	rdfs:label "ParameterValue"@en ;
	rdfs:comment "Provides the value of a given parameter of a detailed model dynamics."^^rdf:XMLLiteral .
<ParameterValue.value> rdf:type rdfs:Property ;
	rdfs:label "value"@en ;
	rdfs:domain <ParameterValue> ;
	rdfs:range xsd:string ;
	rdfs:comment "The value of the parameter."^^rdf:XMLLiteral .
<ParameterValue.ParameterDescriptor> rdf:type rdfs:Property ;
	rdfs:label "ParameterDescriptor"@en ;
	rdfs:domain <ParameterValue> ;
	rdfs:range <ParameterDesctiptor> ;
	rdfs:comment "The parameter descriptor that has this value."^^rdf:XMLLiteral .
<ParameterValue.DetailedModelDynamics> rdf:type rdfs:Property ;
	rdfs:label "DetailedModelDynamics"@en ;
	rdfs:domain <ParameterValue> ;
	rdfs:range <DetailedModelDynamics> ;
	rdfs:comment "The detailed model to which this parameter value applies."^^rdf:XMLLiteral .

<PowerSystemResource> rdf:type rdfs:Class ;
	rdfs:subClassOf <IdentifiedObject> ;
	rdfs:label "PowerSystemResource"@en ;
	rdfs:comment "A power system resource (PSR) can be an item of equipment such as a switch, an equipment container containing many individual items of equipment such as a substation, or an organisational entity such as sub-control area. Power system resources can have measurements associated."^^rdf:XMLLiteral .

<StringIRI> rdf:type rdfs:Datatype ;
	rdfs:label "StringIRI"@en ;
	rdfs:comment "An IRI (Internationalized Resource Identifier) within an RDF graph is a Unicode string that conforms to the syntax defined in RFC 3987.\nThe primitive is serialized as literal without language support.\nIRIs in the RDF abstract syntax must be absolute, and may contain a fragment identifier.\nIRI equality: Two IRIs are equal if and only if they are equivalent under Simple String Comparison according to section 5.1 of [RFC3987]. Further normalization must not be performed when comparing IRIs for equality.\nIRIs are a generalization of URIs [RFC3986] that permits a wider range of Unicode characters. Every absolute URI and URL is an IRI, but not every IRI is an URI. When IRIs are used in operations that are only defined for URIs, they must first be converted according to the mapping defined in section 3.1 of [RFC3987]. A notable example is retrieval over the HTTP protocol. The mapping involves UTF-8 encoding of non-ASCII characters, %-encoding of octets not allowed in URIs, and Punycode-encoding of domain names."^^rdf:XMLLiteral .

<DynamicsFunctionBlock> rdf:type rdfs:Class ;
	rdfs:subClassOf <IdentifiedObject> ;
	rdfs:label "DynamicsFunctionBlock"@en ;
	rdfs:comment "Abstract parent class for all Dynamics function blocks."^^rdf:XMLLiteral .
<DynamicsFunctionBlock.enabled> rdf:type rdfs:Property ;
	rdfs:label "enabled"@en ;
	rdfs:domain <DynamicsFunctionBlock> ;
	rdfs:range xsd:boolean ;
	rdfs:comment "Function block used indicator.\ntrue = use of function block is enabled\nfalse = use of function block is disabled."^^rdf:XMLLiteral .
<DynamicsFunctionBlock.DetailedModelDynamics> rdf:type rdfs:Property ;
	rdfs:label "DetailedModelDynamics"@en ;
	rdfs:domain <DynamicsFunctionBlock> ;
	rdfs:range <DetailedModelDynamics> ;
	rdfs:comment "The detailed model dynamics that has this dynamics function block."^^rdf:XMLLiteral .

<StringFixedLanguage> rdf:type rdfs:Datatype ;
	rdfs:label "StringFixedLanguage"@en ;
	rdfs:comment "A string consisting of a sequence of characters. The character encoding is UTF-8. The string length is unspecified and unlimited.\nThe primitive is serialized as literal without language support."^^rdf:XMLLiteral .

<IRI> rdf:type rdfs:Datatype ;
	rdfs:label "IRI"@en ;
	rdfs:comment "An IRI (Internationalized Resource Identifier) within an RDF graph is a Unicode string that conforms to the syntax defined in RFC 3987.\nThe primitive is serialized as rdf:resource in RDFXML.\nIRIs in the RDF abstract syntax must be absolute, and may contain a fragment identifier.\nIRI equality: Two IRIs are equal if and only if they are equivalent under Simple String Comparison according to section 5.1 of [RFC3987]. Further normalization must not be performed when comparing IRIs for equality.\nIRIs are a generalization of URIs [RFC3986] that permits a wider range of Unicode characters. Every absolute URI and URL is an IRI, but not every IRI is an URI. When IRIs are used in operations that are only defined for URIs, they must first be converted according to the mapping defined in section 3.1 of [RFC3987]. A notable example is retrieval over the HTTP protocol. The mapping involves UTF-8 encoding of non-ASCII characters, %-encoding of octets not allowed in URIs, and Punycode-encoding of domain names."^^rdf:XMLLiteral .

<Equipment> rdf:type rdfs:Class ;
	rdfs:subClassOf <PowerSystemResource> ;
	rdfs:label "Equipment"@en ;
	rdfs:comment "The parts of a power system that are physical devices, electronic or mechanical."^^rdf:XMLLiteral .
<Equipment.DetailedModelDynamics> rdf:type rdfs:Property ;
	rdfs:label "DetailedModelDynamics"@en ;
	rdfs:domain <Equipment> ;
	rdfs:range <DetailedModelDynamics> ;
	rdfs:comment "The detailed model dynamics this models this equipment."^^rdf:XMLLiteral .

<ParameterDesctiptor> rdf:type rdfs:Class ;
	rdfs:subClassOf <DetailedModelDescriptor> ;
	rdfs:label "ParameterDesctiptor"@en ;
	rdfs:comment "Supports definition of one or more parameters of several different datatypes for use by the detailed model.  It describes the parameters used in the equations of the detailed model.\nThe name of the parameter shall be the same as the name used in the equations of the detailed model."^^rdf:XMLLiteral .
<ParameterDesctiptor.ParameterValue> rdf:type rdfs:Property ;
	rdfs:label "ParameterValue"@en ;
	rdfs:domain <ParameterDesctiptor> ;
	rdfs:range <ParameterValue> ;
	rdfs:comment "The value of the parameter descriptor."^^rdf:XMLLiteral .

<DetailedModelDynamics> rdf:type rdfs:Class ;
	rdfs:subClassOf <DynamicsFunctionBlock> ;
	rdfs:label "DetailedModelDynamics"@en ;
	rdfs:comment "The main class that packages all related to this detailed model. This includes all parameters, functions, signals, etc."^^rdf:XMLLiteral .
<DetailedModelDynamics.DetailedModelTypeDynamics> rdf:type rdfs:Property ;
	rdfs:label "DetailedModelTypeDynamics"@en ;
	rdfs:domain <DetailedModelDynamics> ;
	rdfs:range <DetailedModelTypeDynamics> ;
	rdfs:comment "The type of detailed model dynamics that is applied to the detailed model dynamics."^^rdf:XMLLiteral .
<DetailedModelDynamics.ParameterValue> rdf:type rdfs:Property ;
	rdfs:label "ParameterValue"@en ;
	rdfs:domain <DetailedModelDynamics> ;
	rdfs:range <ParameterValue> ;
	rdfs:comment "The value of the parameter for this detailed model dynamics."^^rdf:XMLLiteral .
<DetailedModelDynamics.DynamicsFunctionBlock> rdf:type rdfs:Property ;
	rdfs:label "DynamicsFunctionBlock"@en ;
	rdfs:domain <DetailedModelDynamics> ;
	rdfs:range <DynamicsFunctionBlock> ;
	rdfs:comment "The dynamics function block for this detailed model dynamics."^^rdf:XMLLiteral .
<DetailedModelDynamics.Equipment> rdf:type rdfs:Property ;
	rdfs:label "Equipment"@en ;
	rdfs:domain <DetailedModelDynamics> ;
	rdfs:range <Equipment> ;
	rdfs:comment "The equipment which behaviour this detailed model dynamics represents."^^rdf:XMLLiteral .
