@base <http://iec.ch/TC57/2013/CIM-schema-cim16#> .
@prefix rdf: <http://www.w3.org/1999/02/22-rdf-syntax-ns#> .
@prefix rdfs: <http://www.w3.org/2000/01/rdf-schema#> .
@prefix xsd: <http://www.w3.org/2001/XMLSchema#> .

DetailedModelTypeDynamics rdf:type rdfs:Class ;
	rdfs:subClassOf IdentifiedObject ;
	rdfs:label "DetailedModelTypeDynamics"@en ;
	rdfs:comment "The main class that packages all related to this type of a detailed model. This includes all parameters, functions, signals, etc."^^rdf:XMLLiteral .

DetailedModelDescriptor rdf:type rdfs:Class ;
	rdfs:subClassOf IdentifiedObject ;
	rdfs:label "DetailedModelDescriptor"@en ;
	rdfs:comment "Describes different components of a detailed model."^^rdf:XMLLiteral .

IdentifiedObject rdf:type rdfs:Class ;
	rdfs:label "IdentifiedObject"@en ;
	rdfs:comment "This is a root class to provide common identification for all classes needing identification and naming attributes."^^rdf:XMLLiteral .
IdentifiedObject.description rdf:type rdfs:Property ;
	rdfs:label "description"@en ;
	rdfs:domain IdentifiedObject ;
	rdfs:range xsd:string ;
	rdfs:comment "The description is a free human readable text describing or naming the object. It may be non unique and may not correlate to a naming hierarchy."^^rdf:XMLLiteral .
IdentifiedObject.mRID rdf:type rdfs:Property ;
	rdfs:label "mRID"@en ;
	rdfs:domain IdentifiedObject ;
	rdfs:range xsd:string ;
	rdfs:comment "Master resource identifier issued by a model authority. The mRID is unique within an exchange context. Global uniqueness is easily achieved by using a UUID, as specified in RFC 4122, for the mRID. The use of UUID is strongly recommended.\nFor CIMXML data files in RDF syntax conforming to IEC 61970-552, the mRID is mapped to rdf:ID or rdf:about attributes that identify CIM object elements."^^rdf:XMLLiteral .
IdentifiedObject.name rdf:type rdfs:Property ;
	rdfs:label "name"@en ;
	rdfs:domain IdentifiedObject ;
	rdfs:range xsd:string ;
	rdfs:comment "The name is any free human readable and possibly non unique text naming the object."^^rdf:XMLLiteral .

ParameterValue rdf:type rdfs:Class ;
	rdfs:label "ParameterValue"@en ;
	rdfs:comment "Provides the value of a given parameter of a detailed model dynamics."^^rdf:XMLLiteral .
ParameterValue.value rdf:type rdfs:Property ;
	rdfs:label "value"@en ;
	rdfs:domain ParameterValue ;
	rdfs:range xsd:string ;
	rdfs:comment "The value of the parameter."^^rdf:XMLLiteral .
ParameterValue.ParameterDescriptor rdf:type rdfs:Property ;
	rdfs:label "ParameterDescriptor"@en ;
	rdfs:domain ParameterValue ;
	rdfs:range ParameterDesctiptor ;
	rdfs:comment "The parameter descriptor that has this value."^^rdf:XMLLiteral .
ParameterValue.DetailedModelDynamics rdf:type rdfs:Property ;
	rdfs:label "DetailedModelDynamics"@en ;
	rdfs:domain ParameterValue ;
	rdfs:range DetailedModelDynamics ;
	rdfs:comment "The detailed model to which this parameter value applies."^^rdf:XMLLiteral .

PowerSystemResource rdf:type rdfs:Class ;
	rdfs:subClassOf IdentifiedObject ;
	rdfs:label "PowerSystemResource"@en ;
	rdfs:comment "A power system resource (PSR) can be an item of equipment such as a switch, an equipment container containing many individual items of equipment such as a substation, or an organisational entity such as sub-control area. Power system resources can have measurements associated."^^rdf:XMLLiteral .

StringIRI rdf:type rdfs:Datatype ;
	rdfs:label "StringIRI"@en ;
	rdfs:comment "An IRI (Internationalized Resource Identifier) within an RDF graph is a Unicode string that conforms to the syntax defined in RFC 3987.\nThe primitive is serialized as literal without language support.\nIRIs in the RDF abstract syntax must be absolute, and may contain a fragment identifier.\nIRI equality: Two IRIs are equal if and only if they are equivalent under Simple String Comparison according to section 5.1 of [RFC3987]. Further normalization must not be performed when comparing IRIs for equality.\nIRIs are a generalization of URIs [RFC3986] that permits a wider range of Unicode characters. Every absolute URI and URL is an IRI, but not every IRI is an URI. When IRIs are used in operations that are only defined for URIs, they must first be converted according to the mapping defined in section 3.1 of [RFC3987]. A notable example is retrieval over the HTTP protocol. The mapping involves UTF-8 encoding of non-ASCII characters, %-encoding of octets not allowed in URIs, and Punycode-encoding of domain names."^^rdf:XMLLiteral .

DynamicsFunctionBlock rdf:type rdfs:Class ;
	rdfs:subClassOf IdentifiedObject ;
	rdfs:label "DynamicsFunctionBlock"@en ;
	rdfs:comment "Abstract parent class for all Dynamics function blocks."^^rdf:XMLLiteral .
DynamicsFunctionBlock.enabled rdf:type rdfs:Property ;
	rdfs:label "enabled"@en ;
	rdfs:domain DynamicsFunctionBlock ;
	rdfs:range xsd:boolean ;
	rdfs:comment "Function block used indicator.\ntrue = use of function block is enabled\nfalse = use of function block is disabled."^^rdf:XMLLiteral .

StringFixedLanguage rdf:type rdfs:Datatype ;
	rdfs:label "StringFixedLanguage"@en ;
	rdfs:comment "A string consisting of a sequence of characters. The character encoding is UTF-8. The string length is unspecified and unlimited.\nThe primitive is serialized as literal without language support."^^rdf:XMLLiteral .

IRI rdf:type rdfs:Datatype ;
	rdfs:label "IRI"@en ;
	rdfs:comment "An IRI (Internationalized Resource Identifier) within an RDF graph is a Unicode string that conforms to the syntax defined in RFC 3987.\nThe primitive is serialized as rdf:resource in RDFXML.\nIRIs in the RDF abstract syntax must be absolute, and may contain a fragment identifier.\nIRI equality: Two IRIs are equal if and only if they are equivalent under Simple String Comparison according to section 5.1 of [RFC3987]. Further normalization must not be performed when comparing IRIs for equality.\nIRIs are a generalization of URIs [RFC3986] that permits a wider range of Unicode characters. Every absolute URI and URL is an IRI, but not every IRI is an URI. When IRIs are used in operations that are only defined for URIs, they must first be converted according to the mapping defined in section 3.1 of [RFC3987]. A notable example is retrieval over the HTTP protocol. The mapping involves UTF-8 encoding of non-ASCII characters, %-encoding of octets not allowed in URIs, and Punycode-encoding of domain names."^^rdf:XMLLiteral .

Equipment rdf:type rdfs:Class ;
	rdfs:subClassOf PowerSystemResource ;
	rdfs:label "Equipment"@en ;
	rdfs:comment "The parts of a power system that are physical devices, electronic or mechanical."^^rdf:XMLLiteral .

ParameterDesctiptor rdf:type rdfs:Class ;
	rdfs:subClassOf DetailedModelDescriptor ;
	rdfs:label "ParameterDesctiptor"@en ;
	rdfs:comment "Supports definition of one or more parameters of several different datatypes for use by the detailed model.  It describes the parameters used in the equations of the detailed model.\nThe name of the parameter shall be the same as the name used in the equations of the detailed model."^^rdf:XMLLiteral .

DetailedModelDynamics rdf:type rdfs:Class ;
	rdfs:subClassOf DynamicsFunctionBlock ;
	rdfs:label "DetailedModelDynamics"@en ;
	rdfs:comment "The main class that packages all related to this detailed model. This includes all parameters, functions, signals, etc."^^rdf:XMLLiteral .
DetailedModelDynamics.DetailedModelTypeDynamics rdf:type rdfs:Property ;
	rdfs:label "DetailedModelTypeDynamics"@en ;
	rdfs:domain DetailedModelDynamics ;
	rdfs:range DetailedModelTypeDynamics ;
	rdfs:comment "The type of detailed model dynamics that is applied to the detailed model dynamics."^^rdf:XMLLiteral .
DetailedModelDynamics.DynamicsFunctionBlock rdf:type rdfs:Property ;
	rdfs:label "DynamicsFunctionBlock"@en ;
	rdfs:domain DetailedModelDynamics ;
	rdfs:range DynamicsFunctionBlock ;
	rdfs:comment "The dynamics function block for this detailed model dynamics."^^rdf:XMLLiteral .
DetailedModelDynamics.Equipment rdf:type rdfs:Property ;
	rdfs:label "Equipment"@en ;
	rdfs:domain DetailedModelDynamics ;
	rdfs:range Equipment ;
	rdfs:comment "The equipment which behaviour this detailed model dynamics represents."^^rdf:XMLLiteral .
