@base <http://iec.ch/TC57/2013/CIM-schema-cim16#> .
@prefix rdf: <http://www.w3.org/1999/02/22-rdf-syntax-ns#> .
@prefix rdfs: <http://www.w3.org/2000/01/rdf-schema#> .
@prefix xsd: <http://www.w3.org/2001/XMLSchema#> .

<StringFixedLanguage> rdf:type rdfs:Datatype ;
	rdfs:label "StringFixedLanguage"@en ;
	rdfs:comment "A string consisting of a sequence of characters. The character encoding is UTF-8. The string length is unspecified and unlimited.\nThe primitive is serialized as literal without language support."^^rdf:XMLLiteral .

<ParameterDesctiptor> rdf:type rdfs:Class ;
	rdfs:subClassOf <DetailedModelDescriptor> ;
	rdfs:label "ParameterDesctiptor"@en ;
	rdfs:comment "Supports definition of one or more parameters of several different datatypes for use by the detailed model.  It describes the parameters used in the equations of the detailed model.\nThe name of the parameter shall be the same as the name used in the equations of the detailed model."^^rdf:XMLLiteral .
<ParameterDesctiptor.constraintKind> rdf:type rdfs:Property ;
	rdfs:label "constraintKind"@en ;
	rdfs:domain <ParameterDesctiptor> ;
	rdfs:range xsd:string ;
	rdfs:comment "The kind for the constraint."^^rdf:XMLLiteral .
<ParameterDesctiptor.constraintValue> rdf:type rdfs:Property ;
	rdfs:label "constraintValue"@en ;
	rdfs:domain <ParameterDesctiptor> ;
	rdfs:range xsd:double ;
	rdfs:comment "The value of the constraint. Used in all cases except when constraint kind is \"custom\"."^^rdf:XMLLiteral .
<ParameterDesctiptor.engineeringUnit> rdf:type rdfs:Property ;
	rdfs:label "engineeringUnit"@en ;
	rdfs:domain <ParameterDesctiptor> ;
	rdfs:range xsd:string ;
	rdfs:comment "The engineering unit of the value."^^rdf:XMLLiteral .
<ParameterDesctiptor.kind> rdf:type rdfs:Property ;
	rdfs:label "kind"@en ;
	rdfs:domain <ParameterDesctiptor> ;
	rdfs:range xsd:string ;
	rdfs:comment "The kind of the parameter."^^rdf:XMLLiteral .
<ParameterDesctiptor.referenceCustomConstraint> rdf:type rdfs:Property ;
	rdfs:label "referenceCustomConstraint"@en ;
	rdfs:domain <ParameterDesctiptor> ;
	rdfs:range <IRI> ;
	rdfs:comment "Provides the reference to a custom constraint related to this parameter. It is used for more complex constraints that are not possible to express by attributes constraintKind and constraintValue. The reference is and IRI to a description of the constraint that conform to specific language for describing constraints, e.g. SHACL. "^^rdf:XMLLiteral .
<ParameterDesctiptor.sequenceNumber> rdf:type rdfs:Property ;
	rdfs:label "sequenceNumber"@en ;
	rdfs:domain <ParameterDesctiptor> ;
	rdfs:range xsd:integer ;
	rdfs:comment "Sequence number of the parameter among the set of parameters associated with the related proprietary user-defined model."^^rdf:XMLLiteral .
<ParameterDesctiptor.typicalValue> rdf:type rdfs:Property ;
	rdfs:label "typicalValue"@en ;
	rdfs:domain <ParameterDesctiptor> ;
	rdfs:range xsd:string ;
	rdfs:comment "Typical value for the parameter. The datatype is as specified in attribute valueXSDdatatype."^^rdf:XMLLiteral .
<ParameterDesctiptor.typicalValueRangeMax> rdf:type rdfs:Property ;
	rdfs:label "typicalValueRangeMax"@en ;
	rdfs:domain <ParameterDesctiptor> ;
	rdfs:range xsd:double ;
	rdfs:comment "Maximum value (upper end of the range) of the typical range. "^^rdf:XMLLiteral .
<ParameterDesctiptor.typicalValueRangeMin> rdf:type rdfs:Property ;
	rdfs:label "typicalValueRangeMin"@en ;
	rdfs:domain <ParameterDesctiptor> ;
	rdfs:range xsd:double ;
	rdfs:comment "Minimum value (lower end of the range) of the typical range. "^^rdf:XMLLiteral .
<ParameterDesctiptor.valueXSDdatatype> rdf:type rdfs:Property ;
	rdfs:label "valueXSDdatatype"@en ;
	rdfs:domain <ParameterDesctiptor> ;
	rdfs:range xsd:string ;
	rdfs:comment "The XSD datatype of the value."^^rdf:XMLLiteral .
<ParameterDesctiptor.FunctionDescriptor> rdf:type rdfs:Property ;
	rdfs:label "FunctionDescriptor"@en ;
	rdfs:domain <ParameterDesctiptor> ;
	rdfs:range <FunctionDescriptor> ;
	rdfs:comment "The function descriptor that has parameter descriptor."^^rdf:XMLLiteral .

<InputOutputDescriptor> rdf:type rdfs:Class ;
	rdfs:subClassOf <DetailedModelDescriptor> ;
	rdfs:label "InputOutputDescriptor"@en ;
	rdfs:comment "Describes the inputs and outputs of the functions that describe an detailed model."^^rdf:XMLLiteral .
<InputOutputDescriptor.InputSignal> rdf:type rdfs:Property ;
	rdfs:label "InputSignal"@en ;
	rdfs:domain <InputOutputDescriptor> ;
	rdfs:range <SignalDescriptor> ;
	rdfs:comment "The input signal for this input descriptor."^^rdf:XMLLiteral .
<InputOutputDescriptor.LimiterDescriptor> rdf:type rdfs:Property ;
	rdfs:label "LimiterDescriptor"@en ;
	rdfs:domain <InputOutputDescriptor> ;
	rdfs:range <LimiterDescriptor> ;
	rdfs:comment "The limiter descriptor that has input and output descriptor."^^rdf:XMLLiteral .
<InputOutputDescriptor.OutputSignal> rdf:type rdfs:Property ;
	rdfs:label "OutputSignal"@en ;
	rdfs:domain <InputOutputDescriptor> ;
	rdfs:range <SignalDescriptor> ;
	rdfs:comment "The output signal for this output descriptor."^^rdf:XMLLiteral .
<InputOutputDescriptor.OperatorDescriptor> rdf:type rdfs:Property ;
	rdfs:label "OperatorDescriptor"@en ;
	rdfs:domain <InputOutputDescriptor> ;
	rdfs:range <OperatorDescriptor> ;
	rdfs:comment "The operator descriptor that has input and output descriptor."^^rdf:XMLLiteral .
<InputOutputDescriptor.FunctionDescriptor> rdf:type rdfs:Property ;
	rdfs:label "FunctionDescriptor"@en ;
	rdfs:domain <InputOutputDescriptor> ;
	rdfs:range <FunctionDescriptor> ;
	rdfs:comment "The function descriptor that has this input and output descriptor."^^rdf:XMLLiteral .

<ACDCTerminal> rdf:type rdfs:Class ;
	rdfs:subClassOf <IdentifiedObject> ;
	rdfs:label "ACDCTerminal"@en ;
	rdfs:comment "An electrical connection point (AC or DC) to a piece of conducting equipment. Terminals are connected at physical connection points called connectivity nodes."^^rdf:XMLLiteral .
<ACDCTerminal.SignalDescriptor> rdf:type rdfs:Property ;
	rdfs:label "SignalDescriptor"@en ;
	rdfs:domain <ACDCTerminal> ;
	rdfs:range <SignalDescriptor> ;
	rdfs:comment "The signal descriptor that has a terminal."^^rdf:XMLLiteral .

<DetailedModelDescriptorArtifact> rdf:type rdfs:Class ;
	rdfs:subClassOf <DetailedModelDescriptor> ;
	rdfs:label "DetailedModelDescriptorArtifact"@en ;
	rdfs:comment "An artifact (e.g. file) describing the model. In can be used when reusing existing modules or in the use case where detailed models are already part of a reference library and the DetailedModelDynamics will only need to refer to a model from that library instead of constructing the model in detail."^^rdf:XMLLiteral .
<DetailedModelDescriptorArtifact.equationLanguageKind> rdf:type rdfs:Property ;
	rdfs:label "equationLanguageKind"@en ;
	rdfs:domain <DetailedModelDescriptorArtifact> ;
	rdfs:range xsd:string ;
	rdfs:comment "Describes what kind of language is used to describe the equation."^^rdf:XMLLiteral .
<DetailedModelDescriptorArtifact.equationLanguageTypeOther> rdf:type rdfs:Property ;
	rdfs:label "equationLanguageTypeOther"@en ;
	rdfs:domain <DetailedModelDescriptorArtifact> ;
	rdfs:range xsd:string ;
	rdfs:comment "Defines the language used to describe equations."^^rdf:XMLLiteral .
<DetailedModelDescriptorArtifact.FunctionDescriptor> rdf:type rdfs:Property ;
	rdfs:label "FunctionDescriptor"@en ;
	rdfs:domain <DetailedModelDescriptorArtifact> ;
	rdfs:range <FunctionDescriptor> ;
	rdfs:comment "The functional descriptor that has equation descriptor artifact."^^rdf:XMLLiteral .

<SignalDescriptor> rdf:type rdfs:Class ;
	rdfs:subClassOf <DetailedModelDescriptor> ;
	rdfs:label "SignalDescriptor"@en ;
	rdfs:comment "Describes the signals both internal signals that connect different functions or external signals."^^rdf:XMLLiteral .
<SignalDescriptor.isSignalInverted> rdf:type rdfs:Property ;
	rdfs:label "isSignalInverted"@en ;
	rdfs:domain <SignalDescriptor> ;
	rdfs:range xsd:boolean ;
	rdfs:comment "Indicates if the signal is inverted. True means the signal is inverted, i.e. multiplied by -1. False means the signal is not inverted."^^rdf:XMLLiteral .
<SignalDescriptor.InputDescriptor> rdf:type rdfs:Property ;
	rdfs:label "InputDescriptor"@en ;
	rdfs:domain <SignalDescriptor> ;
	rdfs:range <InputOutputDescriptor> ;
	rdfs:comment "The input of the input descriptor that has this signal descriptor."^^rdf:XMLLiteral .
<SignalDescriptor.OutputDescriptor> rdf:type rdfs:Property ;
	rdfs:label "OutputDescriptor"@en ;
	rdfs:domain <SignalDescriptor> ;
	rdfs:range <InputOutputDescriptor> ;
	rdfs:comment "The output of this input and output desciptor that has a signal descriptor."^^rdf:XMLLiteral .
<SignalDescriptor.ACDCTerminal> rdf:type rdfs:Property ;
	rdfs:label "ACDCTerminal"@en ;
	rdfs:domain <SignalDescriptor> ;
	rdfs:range <ACDCTerminal> ;
	rdfs:comment "Th eterminal for this signal descriptor."^^rdf:XMLLiteral .
<SignalDescriptor.DynamicsFunctionBlock> rdf:type rdfs:Property ;
	rdfs:label "DynamicsFunctionBlock"@en ;
	rdfs:domain <SignalDescriptor> ;
	rdfs:range <DynamicsFunctionBlock> ;
	rdfs:comment "The dynamics function block to which this signal belongs to."^^rdf:XMLLiteral .

<StringIRI> rdf:type rdfs:Datatype ;
	rdfs:label "StringIRI"@en ;
	rdfs:comment "An IRI (Internationalized Resource Identifier) within an RDF graph is a Unicode string that conforms to the syntax defined in RFC 3987.\nThe primitive is serialized as literal without language support.\nIRIs in the RDF abstract syntax must be absolute, and may contain a fragment identifier.\nIRI equality: Two IRIs are equal if and only if they are equivalent under Simple String Comparison according to section 5.1 of [RFC3987]. Further normalization must not be performed when comparing IRIs for equality.\nIRIs are a generalization of URIs [RFC3986] that permits a wider range of Unicode characters. Every absolute URI and URL is an IRI, but not every IRI is an URI. When IRIs are used in operations that are only defined for URIs, they must first be converted according to the mapping defined in section 3.1 of [RFC3987]. A notable example is retrieval over the HTTP protocol. The mapping involves UTF-8 encoding of non-ASCII characters, %-encoding of octets not allowed in URIs, and Punycode-encoding of domain names."^^rdf:XMLLiteral .

<DynamicsFunctionBlock> rdf:type rdfs:Class ;
	rdfs:subClassOf <IdentifiedObject> ;
	rdfs:label "DynamicsFunctionBlock"@en ;
	rdfs:comment "Abstract parent class for all Dynamics function blocks."^^rdf:XMLLiteral .
<DynamicsFunctionBlock.SignalDescriptor> rdf:type rdfs:Property ;
	rdfs:label "SignalDescriptor"@en ;
	rdfs:domain <DynamicsFunctionBlock> ;
	rdfs:range <SignalDescriptor> ;
	rdfs:comment "The signal which relates to this dynamics function block."^^rdf:XMLLiteral .

<FunctionDescriptor> rdf:type rdfs:Class ;
	rdfs:subClassOf <DetailedModelDescriptor> ;
	rdfs:label "FunctionDescriptor"@en ;
	rdfs:comment "Describes a function part of the detailed model."^^rdf:XMLLiteral .
<FunctionDescriptor.describedByArtifact> rdf:type rdfs:Property ;
	rdfs:label "describedByArtifact"@en ;
	rdfs:domain <FunctionDescriptor> ;
	rdfs:range xsd:boolean ;
	rdfs:comment "Identifies if the function descriptor is described by an artifact. If true, the function is described by an artifact. If false the equation shall be described by the attribute equation."^^rdf:XMLLiteral .
<FunctionDescriptor.equation> rdf:type rdfs:Property ;
	rdfs:label "equation"@en ;
	rdfs:domain <FunctionDescriptor> ;
	rdfs:range xsd:string ;
	rdfs:comment "Mathematical expression of the function in the specified language. A function can be e.g. first-order lag element, more complex transfer function, etc."^^rdf:XMLLiteral .
<FunctionDescriptor.equationLanguageKind> rdf:type rdfs:Property ;
	rdfs:label "equationLanguageKind"@en ;
	rdfs:domain <FunctionDescriptor> ;
	rdfs:range xsd:string ;
	rdfs:comment "Describes what kind of language is used to describe the equation."^^rdf:XMLLiteral .
<FunctionDescriptor.initialConditionsEquation> rdf:type rdfs:Property ;
	rdfs:label "initialConditionsEquation"@en ;
	rdfs:domain <FunctionDescriptor> ;
	rdfs:range xsd:string ;
	rdfs:comment "Mathematical expression (in the specified language) of the initial conditions of the function descriptor. "^^rdf:XMLLiteral .
<FunctionDescriptor.ParameterDescriptor> rdf:type rdfs:Property ;
	rdfs:label "ParameterDescriptor"@en ;
	rdfs:domain <FunctionDescriptor> ;
	rdfs:range <ParameterDesctiptor> ;
	rdfs:comment "The parameter descriptor for this function descriptor."^^rdf:XMLLiteral .
<FunctionDescriptor.InputOutputDescriptor> rdf:type rdfs:Property ;
	rdfs:label "InputOutputDescriptor"@en ;
	rdfs:domain <FunctionDescriptor> ;
	rdfs:range <InputOutputDescriptor> ;
	rdfs:comment "The input and output descriptor of this function descriptor."^^rdf:XMLLiteral .
<FunctionDescriptor.EquationDescriptorArtifact> rdf:type rdfs:Property ;
	rdfs:label "EquationDescriptorArtifact"@en ;
	rdfs:domain <FunctionDescriptor> ;
	rdfs:range <DetailedModelDescriptorArtifact> ;
	rdfs:comment "The equation descriptor artifact for this function descriptor."^^rdf:XMLLiteral .
<FunctionDescriptor.LowerLimit> rdf:type rdfs:Property ;
	rdfs:label "LowerLimit"@en ;
	rdfs:domain <FunctionDescriptor> ;
	rdfs:range <LimiterDescriptor> ;
	rdfs:comment "The lower limit of the limiter descriptor."^^rdf:XMLLiteral .
<FunctionDescriptor.UpperLimit> rdf:type rdfs:Property ;
	rdfs:label "UpperLimit"@en ;
	rdfs:domain <FunctionDescriptor> ;
	rdfs:range <LimiterDescriptor> ;
	rdfs:comment "The upper limit of the limiter descriptor."^^rdf:XMLLiteral .

<IRI> rdf:type rdfs:Datatype ;
	rdfs:label "IRI"@en ;
	rdfs:comment "An IRI (Internationalized Resource Identifier) within an RDF graph is a Unicode string that conforms to the syntax defined in RFC 3987.\nThe primitive is serialized as rdf:resource in RDFXML.\nIRIs in the RDF abstract syntax must be absolute, and may contain a fragment identifier.\nIRI equality: Two IRIs are equal if and only if they are equivalent under Simple String Comparison according to section 5.1 of [RFC3987]. Further normalization must not be performed when comparing IRIs for equality.\nIRIs are a generalization of URIs [RFC3986] that permits a wider range of Unicode characters. Every absolute URI and URL is an IRI, but not every IRI is an URI. When IRIs are used in operations that are only defined for URIs, they must first be converted according to the mapping defined in section 3.1 of [RFC3987]. A notable example is retrieval over the HTTP protocol. The mapping involves UTF-8 encoding of non-ASCII characters, %-encoding of octets not allowed in URIs, and Punycode-encoding of domain names."^^rdf:XMLLiteral .

<DetailedModelDocumentationArtifact> rdf:type rdfs:Class ;
	rdfs:subClassOf <DetailedModelDescriptor> ;
	rdfs:label "DetailedModelDocumentationArtifact"@en ;
	rdfs:comment "An artifact describing the model. For instance documentation containing block diagrams, results from reference implementation, etc."^^rdf:XMLLiteral .

<IdentifiedObject> rdf:type rdfs:Class ;
	rdfs:label "IdentifiedObject"@en ;
	rdfs:comment "This is a root class to provide common identification for all classes needing identification and naming attributes."^^rdf:XMLLiteral .
<IdentifiedObject.description> rdf:type rdfs:Property ;
	rdfs:label "description"@en ;
	rdfs:domain <IdentifiedObject> ;
	rdfs:range xsd:string ;
	rdfs:comment "The description is a free human readable text describing or naming the object. It may be non unique and may not correlate to a naming hierarchy."^^rdf:XMLLiteral .
<IdentifiedObject.mRID> rdf:type rdfs:Property ;
	rdfs:label "mRID"@en ;
	rdfs:domain <IdentifiedObject> ;
	rdfs:range xsd:string ;
	rdfs:comment "Master resource identifier issued by a model authority. The mRID is unique within an exchange context. Global uniqueness is easily achieved by using a UUID, as specified in RFC 4122, for the mRID. The use of UUID is strongly recommended.\nFor CIMXML data files in RDF syntax conforming to IEC 61970-552, the mRID is mapped to rdf:ID or rdf:about attributes that identify CIM object elements."^^rdf:XMLLiteral .
<IdentifiedObject.name> rdf:type rdfs:Property ;
	rdfs:label "name"@en ;
	rdfs:domain <IdentifiedObject> ;
	rdfs:range xsd:string ;
	rdfs:comment "The name is any free human readable and possibly non unique text naming the object."^^rdf:XMLLiteral .

<OperatorDescriptor> rdf:type rdfs:Class ;
	rdfs:subClassOf <DetailedModelDescriptor> ;
	rdfs:label "OperatorDescriptor"@en ;
	rdfs:comment "Describes the operator that connects different signals."^^rdf:XMLLiteral .
<OperatorDescriptor.logicalKind> rdf:type rdfs:Property ;
	rdfs:label "logicalKind"@en ;
	rdfs:domain <OperatorDescriptor> ;
	rdfs:range xsd:string ;
	rdfs:comment "Logical kind of the operator. Used only if operatorKind is set to OperatorDescriptorKind.logical."^^rdf:XMLLiteral .
<OperatorDescriptor.operatorKind> rdf:type rdfs:Property ;
	rdfs:label "operatorKind"@en ;
	rdfs:domain <OperatorDescriptor> ;
	rdfs:range xsd:string ;
	rdfs:comment "Kinds of operator."^^rdf:XMLLiteral .
<OperatorDescriptor.InputOutputDescriptor> rdf:type rdfs:Property ;
	rdfs:label "InputOutputDescriptor"@en ;
	rdfs:domain <OperatorDescriptor> ;
	rdfs:range <InputOutputDescriptor> ;
	rdfs:comment "The input and otput descriptor that belongs to the  operator descriptor."^^rdf:XMLLiteral .

<DetailedModelDescriptor> rdf:type rdfs:Class ;
	rdfs:subClassOf <IdentifiedObject> ;
	rdfs:label "DetailedModelDescriptor"@en ;
	rdfs:comment "Describes different components of a detailed model."^^rdf:XMLLiteral .
<DetailedModelDescriptor.DetailedModelTypeDynamics> rdf:type rdfs:Property ;
	rdfs:label "DetailedModelTypeDynamics"@en ;
	rdfs:domain <DetailedModelDescriptor> ;
	rdfs:range <DetailedModelTypeDynamics> ;
	rdfs:comment "The detailed model type dynamics that has detailed model descriptor."^^rdf:XMLLiteral .

<LimiterDescriptor> rdf:type rdfs:Class ;
	rdfs:subClassOf <DetailedModelDescriptor> ;
	rdfs:label "LimiterDescriptor"@en ;
	rdfs:comment "Describes a limiter part of the detailed model."^^rdf:XMLLiteral .
<LimiterDescriptor.InputOutputDescriptor> rdf:type rdfs:Property ;
	rdfs:label "InputOutputDescriptor"@en ;
	rdfs:domain <LimiterDescriptor> ;
	rdfs:range <InputOutputDescriptor> ;
	rdfs:comment "The input and output descriptor that belongs to the limiter descriptor."^^rdf:XMLLiteral .
<LimiterDescriptor.LowerLimitFunction> rdf:type rdfs:Property ;
	rdfs:label "LowerLimitFunction"@en ;
	rdfs:domain <LimiterDescriptor> ;
	rdfs:range <FunctionDescriptor> ;
	rdfs:comment "The function fo the lower limit."^^rdf:XMLLiteral .
<LimiterDescriptor.UpperLimitFunction> rdf:type rdfs:Property ;
	rdfs:label "UpperLimitFunction"@en ;
	rdfs:domain <LimiterDescriptor> ;
	rdfs:range <FunctionDescriptor> ;
	rdfs:comment "The function for the upper limit."^^rdf:XMLLiteral .

<DetailedModelTypeDynamics> rdf:type rdfs:Class ;
	rdfs:subClassOf <IdentifiedObject> ;
	rdfs:label "DetailedModelTypeDynamics"@en ;
	rdfs:comment "The main class that packages all related to this type of a detailed model. This includes all parameters, functions, signals, etc."^^rdf:XMLLiteral .
<DetailedModelTypeDynamics.DetailedModelDescriptor> rdf:type rdfs:Property ;
	rdfs:label "DetailedModelDescriptor"@en ;
	rdfs:domain <DetailedModelTypeDynamics> ;
	rdfs:range <DetailedModelDescriptor> ;
	rdfs:comment "The detailed model descriptor that is part of the detailed model type dynamics."^^rdf:XMLLiteral .
